Move [list_to_imap] to Helpers/

src/Helpers/Map.v
@@ -22,3 +22,92 @@ Section map.
   Qed.
 
 End map.
+
+(** turn a list into a gmap from its indices to values *)
+Definition list_to_imap {A} (l: list A) : gmap nat A :=
+  list_to_map (imap (λ i x, (i, x)) l).
+
+Theorem imap_NoDup {A B} (f: nat → A → B) (l: list A) :
+  (∀ i1 x1 i2 x2,
+      i1 ≠ i2 →
+      l !! i1 = Some x1 →
+      l !! i2 = Some x2 →
+      f i1 x1 ≠ f i2 x2) →
+  NoDup (imap f l).
+Proof.
+  revert f.
+  induction l as [|x l]; simpl; intros f Hfneq.
+  - constructor.
+  - constructor.
+    + intros Helem%elem_of_lookup_imap_1.
+      destruct Helem as (i'&x'&[Heq Hlookup]).
+      apply Hfneq in Heq; eauto.
+    + apply IHl; intros.
+      eapply Hfneq; eauto.
+Qed.
+
+Theorem lookup_list_to_imap_Some {A} l (i: nat) (x: A) :
+  l !! i = Some x <-> list_to_imap l !! i = Some x.
+Proof.
+  rewrite /list_to_imap.
+  revert i.
+  induction l; simpl; intros.
+  - auto.
+  - destruct i; simpl.
+    + rewrite lookup_insert //.
+    + rewrite -> lookup_insert_ne by lia.
+      rewrite IHl.
+      split.
+      * intros Helem%elem_of_list_to_map_2%elem_of_lookup_imap_1.
+        destruct Helem as (i'&x'&[Heq Hlookup]).
+        inversion Heq; subst; clear Heq.
+        apply elem_of_list_to_map_1.
+        { rewrite fmap_imap.
+          simpl.
+          apply imap_NoDup; intros; simpl.
+          auto. }
+        change (S i', x') with (((λ (i : nat) (x : A), (i, x)) ∘ S) i' x').
+        eapply elem_of_lookup_imap_2; eauto.
+      * intros Helem%elem_of_list_to_map_2%elem_of_lookup_imap_1.
+        destruct Helem as (i'&x'&[Heq Hlookup]).
+        inversion Heq; subst; clear Heq.
+        apply elem_of_list_to_map_1.
+        { rewrite fmap_imap.
+          simpl.
+          apply imap_NoDup; intros; simpl.
+          auto. }
+        eapply elem_of_lookup_imap_2; eauto.
+Qed.
+
+(** a theorem that essentially fully characterizes [list_to_imap l] in terms of
+    lookups (one the one hand gmap lookups, on the other list lookup) *)
+Theorem lookup_list_to_imap {A} (l: list A) (i: nat) :
+  list_to_imap l !! i = l !! i.
+Proof.
+  destruct (l !! i) eqn:Hl.
+  - apply lookup_list_to_imap_Some in Hl; auto.
+  - destruct (list_to_imap l !! i) eqn:Himapl; auto.
+    apply lookup_list_to_imap_Some in Himapl; congruence.
+Qed.
+
+Theorem list_to_imap_app1 {A} (l: list A) (y: A) :
+  list_to_imap (l ++ [y]) = <[length l := y]> (list_to_imap l).
+Proof.
+  apply map_eq_iff; intros.
+  rewrite lookup_list_to_imap.
+  destruct (decide (i < length l)%nat);
+    [ | destruct (decide (i = length l)); subst ].
+  - rewrite -> lookup_app_l by lia.
+    rewrite -> lookup_insert_ne by lia.
+    rewrite lookup_list_to_imap //.
+  - rewrite -> lookup_app_r by lia.
+    replace (length l - length l)%nat with 0%nat by lia.
+    rewrite /= lookup_insert //.
+  - rewrite -> lookup_insert_ne by lia.
+    rewrite lookup_list_to_imap.
+    rewrite -> lookup_app_r by lia.
+    replace (i - length l)%nat with (S (i - length l - 1))%nat by lia; simpl.
+    rewrite lookup_nil.
+    rewrite -> lookup_ge_None_2 by lia.
+    auto.
+Qed.
